% LineEqualityProof.tex
% This file contains the proof

\begin{proofbox}
Let \( L_1 = \{ t\bar{p} + (1 - t)\bar{q} : t \in \mathbb{R} \} \)  
and \( L_2 = \{ s\bar{a} + (1 - s)\bar{b} : s \in \mathbb{R} \} \).  

Assume that \( L_1 \) and \( L_2 \) intersect at two distinct points, say \( \bar{u} \) and \( \bar{v} \),  
with \( \bar{u} \ne \bar{v} \). Let \( L \) be the line through \( \bar{u} \) and \( \bar{v} \).  

We shall show that \( L_1 = L = L_2 \).  

\vspace{1em}

Since \( \bar{u}, \bar{v} \in L_1 \), there exist \( t_0, t_1 \in \mathbb{R} \) such that  
\[
\bar{u} = t_0\bar{p} + (1 - t_0)\bar{q}, \quad
\bar{v} = t_1\bar{p} + (1 - t_1)\bar{q}.
\]
Since \( \bar{u} \ne \bar{v} \), it follows that \( t_0 \ne t_1 \).  

\vspace{1em}

Now consider a point
\[
\bar{x} = r(t_0\bar{p} + (1 - t_0)\bar{q}) + (1 - r)(t_1\bar{p} + (1 - t_1)\bar{q}).
\]
By the properties of vector addition and scalar multiplication,
\begin{align*}
\bar{x}
&= \big( rt_0 + (1 - r)t_1 \big) \bar{p}
+ \big( r(1 - t_0) + (1 - r)(1 - t_1) \big) \bar{q} \\
&= \big( rt_0 + t_1 - rt_1 \big) \bar{p}
+ \big( r - rt_0 + 1 - r - (1 - t_1) \big) \bar{q} \\
&= \big( rt_0 + t_1 - rt_1 \big) \bar{p}
+ \big( 1 - (rt_0 + t_1 - rt_1) \big) \bar{q}.
\end{align*}
Hence \( \bar{x} \in L_1 \). But \( \bar{x} \) was a point on the line through \( \bar{u} \) and \( \bar{v} \),  
so this shows every point on the line \( L \) lies in \( L_1 \).  

\vspace{1em}

Now, using the identities:
\[
\bar{u} = t_0\bar{p} + (1 - t_0)\bar{q}, \quad
\bar{v} = t_1\bar{p} + (1 - t_1)\bar{q},
\]
we multiply both by \( t_1 \) and \( t_0 \), respectively:
\begin{align*}
t_1\bar{u} &= t_1t_0\bar{p} + t_1(1 - t_0)\bar{q} \tag{A} \\
t_0\bar{v} &= t_0t_1\bar{p} + t_0(1 - t_1)\bar{q} \tag{B}
\end{align*}


\end{proofbox}
\begin{proofbox}
Subtracting (B) from (A):
\begin{align*}
t_1\bar{u} - t_0\bar{v}
&= t_1(1 - t_0)\bar{q} - t_0(1 - t_1)\bar{q} \\
&= \big( t_1 - t_0 \big)\bar{q} \\
\Rightarrow \quad \bar{q} &= \frac{t_1\bar{u} - t_0\bar{v}}{t_1 - t_0}
= \frac{t_0}{t_1 - t_0} \bar{u} - \frac{t_1}{t_1 - t_0} \bar{v} \tag{C}
\end{align*}

\vspace{1em}


Likewise, observe:
\begin{align*}
\bar{u} - \bar{v}
&= (t_0 - t_1)\bar{p} + (1 - t_0 - (1 - t_1))\bar{q} \\
&= (t_0 - t_1)\bar{p} + (t_1 - t_0)\bar{q} \\
&= (t_0 - t_1)(\bar{p} - \bar{q}) \\
\Rightarrow \quad \bar{p}
&= \frac{1 - t_0}{t_0 - t_1} \bar{u} - \frac{1 - t_1}{t_0 - t_1} \bar{v} \tag{D}
\end{align*}
    
Now suppose that \( \bar{y} \in L_1 \). Then \( \bar{y} = t\bar{p} + (1 - t)\bar{q} \) for some \( t \in \mathbb{R} \).  
Substitute from (C) and (D):
\begin{align*}
\bar{y}
&= t\left( \frac{1 - t_0}{t_0 - t_1} \bar{u} - \frac{1 - t_1}{t_0 - t_1} \bar{v} \right)
+ (1 - t) \left( \frac{t_0}{t_1 - t_0} \bar{u} - \frac{t_1}{t_1 - t_0} \bar{v} \right) \\
&= \left( \frac{t(1 - t_0)}{t_0 - t_1} + \frac{(1 - t)t_0}{t_0 - t_1} \right) \bar{u}
+ \left( -\frac{t(1 - t_1)}{t_0 - t_1} - \frac{(1 - t)t_1}{t_0 - t_1} \right) \bar{v} \\
&= \frac{t - t_1}{t_0 - t_1} \bar{u}
+ \left( 1 - \frac{t - t_1}{t_0 - t_1} \right) \bar{v}.
\end{align*}

Thus \( \bar{y} \in L \). So every point on \( L_1 \) lies on \( L \), i.e., \( L_1 \subseteq L \).  
By symmetry, the same argument shows \( L_2 \subseteq L \).  
Hence, \( L_1 = L = L_2 \).  
\hfill \( \qed \)
\end{proofbox}
